$$
\frac{\partial \mathcal{L}}{\partial q_i} - \frac{d}{dt}\frac{\partial \mathcal{L}}{\partial \dot{q_i}} = 0
$$


$$ A = \int_{t_0}^{t_1} f(x(t), \dot{x}(t)) dt $$

$$
\delta A = \int_{t_0}^{t_1} \delta f(x, \dot{x})dt = 0
$$

\begin{align*}
    \frac{\partial}{\partial x_i} f_i &=
    \frac{\partial}{\partial x_i} f \left(x_i, \frac{x_i - x_{i-1}}{\varepsilon}\right) \\
    &= \frac{\partial f_i}{\partial x_i} + \frac{\partial v_i}{\partial x_i} \frac{\partial f_i}{\partial v_i} \\
    &= \frac{\partial f_i}{\partial x_i} + \frac{1}{\varepsilon} \frac{\partial f_i}{\partial v_i}
\end{align*}

\begin{align}
    x &= X \cos(\omega t) + Y \sin(\omega t) \notag \\
    y &= X \sin(\omega t) - Y \cos(\omega t) \label{eq:rotation}
\end{align}

$$
\delta \mathcal{L}(\vec{q}, \vec{\dot{q}}) = \sum_i \left( \dot{p}_i \delta q_i
+ p_i \delta \dot{q}_i \right)
$$

\begin{equation}
    \frac{d \mathcal{L}(\vec{q}, \vec{\dot{q}})}{dt} = \sum_i \left\{ \frac{\partial \mathcal{L}}{\partial q_i} \dot{q}_i
    + \frac{\partial \mathcal{L}}{\partial \dot{q}_i} \ddot{q}_i \right\} \label{eq:tsym}
\end{equation}

$ \mathbf{u} \circletimes \mathbf{v} $

$$
P =
\frac{1}{2\varepsilon}
\begin{pmatrix}
0 & i & 0 & \cdots & 0 \\
-i & 0 & i & \cdots & 0 \\
0 & -i & 0 & \cdots & 0 \\
\vdots & \vdots & \vdots & \ddots & \vdots \\
0 & 0 & 0 & \cdots & 0
\end{pmatrix}
$$
